



$-9 \div 1 =$	$1 \times (-7) =$
$-8 - (-6) =$	$-72 \div (-9) =$
$-5 - 8 =$	$-4 + 7 =$
$-6 + (-4) =$	$2 + (-1) =$
$-7 - (-4) =$	$-48 \div (-8) =$
$14 \div (-2) =$	$1 - 1 =$
$7 + (-3) =$	$6 + (-2) =$
$1 \times 6 =$	$1 \times (-4) =$
$9 - 9 =$	$7 - 8 =$
$8 - (-7) =$	$-5 + 9 =$
$4 \times (-9) =$	$5 + 7 =$
$1 \times (-9) =$	$-42 \div (-6) =$
$-4 \times 2 =$	$9 \times (-4) =$
$-7 - (-1) =$	$4 \times (-3) =$
$9 + 3 =$	$-4 + (-8) =$
$1 - 3 =$	$-3 - (-2) =$
$54 \div (-9) =$	$-9 + 8 =$
$-1 + 8 =$	$-6 - 7 =$
$4 + (-6) =$	$5 \times (-3) =$
$-20 \div (-5) =$	$6 - 6 =$
$49 \div (-7) =$	$2 \div 2 =$
$2 + 8 =$	$-3 + (-3) =$
$-8 + (-2) =$	$-2 \times 2 =$
$-2 \times 7 =$	$-3 - 1 =$
$-8 \times 1 =$	$8 \times (-8) =$